theories/lifetime/tl_borrow.v
@@ -1,32 +1,32 @@
-From lrust Require Export lifetime.
+From lrust.lifetime Require Export derived.
 From iris.base_logic.lib Require Export thread_local.
 From iris.proofmode Require Import tactics.
 
-Definition tl_borrow `{invG Σ, lifetimeG Σ, thread_localG Σ}
-           (κ : lifetime) (tid : thread_id) (N : namespace) (P : iProp Σ) :=
-  (∃ i, idx_borrow κ i P ∗ tl_inv tid N (idx_borrow_own 1 i))%I.
+Definition tl_bor `{invG Σ, lftG Σ, thread_localG Σ}
+           (κ : lft) (tid : thread_id) (N : namespace) (P : iProp Σ) :=
+  (∃ i, idx_bor κ i P ∗ tl_inv tid N (idx_bor_own 1 i))%I.
 
-Notation "&tl{ κ , tid , N } P" := (tl_borrow κ tid N P)
+Notation "&tl{ κ , tid , N } P" := (tl_bor κ tid N P)
   (format "&tl{ κ , tid , N } P", at level 20, right associativity) : uPred_scope.
 
-Section tl_borrow.
-  Context `{invG Σ, lifetimeG Σ, thread_localG Σ}
+Section tl_bor.
+  Context `{invG Σ, lftG Σ, thread_localG Σ}
           (tid : thread_id) (N : namespace) (P : iProp Σ).
 
-  Global Instance tl_borrow_persistent κ : PersistentP (&tl{κ,tid,N} P) := _.
-  Global Instance tl_borrow_proper κ :
-    Proper ((⊣⊢) ==> (⊣⊢)) (tl_borrow κ tid N).
+  Global Instance tl_bor_persistent κ : PersistentP (&tl{κ,tid,N} P) := _.
+  Global Instance tl_bor_proper κ :
+    Proper ((⊣⊢) ==> (⊣⊢)) (tl_bor κ tid N).
   Proof.
     intros P1 P2 EQ. apply uPred.exist_proper. intros i. by rewrite EQ.
   Qed.
 
-  Lemma borrow_tl κ E : ↑lftN ⊆ E → &{κ}P ={E}=∗ &tl{κ,tid,N}P.
+  Lemma bor_tl κ E : ↑lftN ⊆ E → &{κ}P ={E}=∗ &tl{κ,tid,N}P.
   Proof.
-    iIntros (?) "HP". unfold borrow. iDestruct "HP" as (i) "[#? Hown]".
+    iIntros (?) "HP". rewrite bor_unfold_idx. iDestruct "HP" as (i) "[#? Hown]".
     iExists i. iFrame "#". iApply (tl_inv_alloc tid E N with "[Hown]"). auto.
   Qed.
 
-  Lemma tl_borrow_acc q κ E F :
+  Lemma tl_bor_acc q κ E F :
     ↑lftN ⊆ E → ↑tlN ⊆ E → ↑N ⊆ F →
     lft_ctx -∗ &tl{κ,tid,N}P -∗ q.[κ] -∗ tl_own tid F ={E}=∗
             ▷P ∗ tl_own tid (F ∖ ↑N) ∗
@@ -35,17 +35,17 @@ Section tl_borrow.
     iIntros (???) "#LFT#HP Hκ Htlown".
     iDestruct "HP" as (i) "(#Hpers&#Hinv)".
     iMod (tl_inv_open with "Hinv Htlown") as "(>Hown&Htlown&Hclose)"; try done.
-    iMod (idx_borrow_acc with "LFT Hpers Hown Hκ") as "[HP Hclose']". done.
+    iMod (idx_bor_acc with "LFT Hpers Hown Hκ") as "[HP Hclose']". done.
     iIntros "{$HP $Htlown}!>HP Htlown".
     iMod ("Hclose'" with "HP") as "[Hown $]". iApply "Hclose". by iFrame.
   Qed.
 
-  Lemma tl_borrow_shorten κ κ': κ ⊑ κ' -∗ &tl{κ'|tid|N}P -∗ &tl{κ,tid,N}P.
+  Lemma tl_bor_shorten κ κ': κ ⊑ κ' -∗ &tl{κ',tid,N}P -∗ &tl{κ,tid,N}P.
   Proof.
     iIntros "Hκκ' H". iDestruct "H" as (i) "[??]". iExists i. iFrame.
-    iApply (idx_borrow_shorten with "Hκκ' H").
+    iApply (idx_bor_shorten with "Hκκ' H").
   Qed.
 
-End tl_borrow.
+End tl_bor.
 
-Typeclasses Opaque tl_borrow.
+Typeclasses Opaque tl_bor.
